Prove sim_memory_strong_cap

src/localdrf/CapMap.v
@@ -274,14 +274,14 @@ End CONCRETEIDENT.
 
 Section CAPFLEX.
 
-  Inductive cap_flex (mem1 mem2: Memory.t) (newmax: TimeMap.t): Prop :=
+  Inductive cap_flex (mem1 mem2: Memory.t) (tm: TimeMap.t): Prop :=
   | cap_flex_intro
       (SOUND: Memory.le mem1 mem2)
       (MIDDLE: forall loc from1 to1 from2 to2
                       (ADJ: Memory.adjacent loc from1 to1 from2 to2 mem1)
                       (TO: Time.lt to1 from2),
           Memory.get loc from2 mem2 = Some (to1, Message.reserve))
-      (BACK: forall loc, Memory.get loc (newmax loc) mem2 =
+      (BACK: forall loc, Memory.get loc (tm loc) mem2 =
                          Some (Memory.max_ts loc mem1, Message.reserve))
       (COMPLETE: forall loc from to msg
                         (GET1: Memory.get loc to mem1 = None)
@@ -291,12 +291,12 @@ Section CAPFLEX.
   Hint Constructors cap_flex.
 
   Lemma cap_flex_inv
-        mem1 mem2 newmax
+        mem1 mem2 tm
         loc from to msg
         (CLOSED: Memory.closed mem1)
-        (CAP: cap_flex mem1 mem2 newmax)
+        (CAP: cap_flex mem1 mem2 tm)
         (GET: Memory.get loc to mem2 = Some (from, msg))
-        (NEWMAX: forall loc, Time.lt (Memory.max_ts loc mem1) (newmax loc))
+        (TM: forall loc, Time.lt (Memory.max_ts loc mem1) (tm loc))
     :
     Memory.get loc to mem1 = Some (from, msg) \/
     (Memory.get loc to mem1 = None /\
@@ -306,7 +306,7 @@ Section CAPFLEX.
         msg = Message.reserve) \/
     (Memory.get loc to mem1 = None /\
      from = Memory.max_ts loc mem1 /\
-     to = newmax loc /\
+     to = tm loc /\
      msg = Message.reserve).
   Proof.
     inv CAP. move GET at bottom.
@@ -373,19 +373,19 @@ Section CAPFLEX.
       exploit Memory.get_disjoint; [exact GET|exact BACK|..]. i. des.
       { subst. esplits; eauto. }
       exfalso.
-      destruct (Time.le_lt_dec to (newmax loc)).
+      destruct (Time.le_lt_dec to (tm loc)).
       + apply (x1 to); econs; ss. refl.
-      + apply (x1 (newmax loc)); econs; s;
-          eauto using NEWMAX; try refl.
+      + apply (x1 (tm loc)); econs; s;
+          eauto using TM; try refl.
         econs. ss.
   Qed.
 
   Lemma cap_flex_exists
-        mem1 newmax
+        mem1 tm
         (CLOSED1: Memory.closed mem1)
-        (NEWMAX: forall loc, Time.lt (Memory.max_ts loc mem1) (newmax loc))
+        (TM: forall loc, Time.lt (Memory.max_ts loc mem1) (tm loc))
     :
-      exists mem2, (<<CAP: cap_flex mem1 mem2 newmax>>).
+      exists mem2, (<<CAP: cap_flex mem1 mem2 tm>>).
   Proof.
     hexploit Memory.cap_exists; eauto. i. des.
     hexploit (@choice
@@ -393,7 +393,7 @@ Section CAPFLEX.
                 (fun loc cell =>
                    forall ts,
                      Cell.get ts cell =
-                     if (Time.eq_dec ts (newmax loc))
+                     if (Time.eq_dec ts (tm loc))
                      then Some (Memory.max_ts loc mem1, Message.reserve)
                      else if (Time.eq_dec ts (Time.incr (Memory.max_ts loc mem1)))
                           then None
@@ -401,7 +401,7 @@ Section CAPFLEX.
     { intros loc.
       hexploit (@Cell.remove_exists (mem2 loc)).
       { inv CAP. eapply BACK. } i. des.
-      hexploit (@Cell.add_exists cell2 (Memory.max_ts loc mem1) (newmax loc) Message.reserve).
+      hexploit (@Cell.add_exists cell2 (Memory.max_ts loc mem1) (tm loc) Message.reserve).
       { i. erewrite Cell.remove_o in GET2; eauto. des_ifs.
         eapply Memory.cap_inv in GET2; eauto. des; clarify.
         { symmetry. eapply interval_le_disjoint.
@@ -422,7 +422,7 @@ Section CAPFLEX.
     { ii. unfold Memory.get. rewrite SPEC. des_ifs.
       { eapply Memory.max_ts_spec in LHS. des.
         exfalso. eapply Time.lt_strorder. eapply TimeFacts.lt_le_lt.
-        { eapply NEWMAX. }
+        { eapply TM. }
         { eapply MAX. }
       }
       { eapply Memory.max_ts_spec in LHS. des.
@@ -476,6 +476,96 @@ Section CAPFLEX.
     inv CAP. econs; eauto.
   Qed.
 
+  Lemma cap_flex_max_ts mem1 mem2 tm
+        (CLOSED: Memory.closed mem1)
+        (CAP: cap_flex mem1 mem2 tm)
+        (TM: forall loc, Time.lt (Memory.max_ts loc mem1) (tm loc))
+    :
+      forall loc,
+        Memory.max_ts loc mem2 = tm loc.
+  Proof.
+    i. dup CAP. inv CAP0. specialize (BACK loc).
+    exploit Memory.max_ts_spec; try exact BACK. i. des.
+    apply TimeFacts.antisym; ss.
+    destruct (Time.le_lt_dec (Memory.max_ts loc mem2) (tm loc)); ss.
+    exploit cap_flex_inv; try exact GET; eauto. i. des.
+    - exploit Memory.max_ts_spec; try exact x0. i. des.
+      exploit TimeFacts.lt_le_lt; try exact l; try exact MAX0. i.
+      specialize (TM loc). rewrite x1 in TM. timetac.
+    - inv x1. exploit Memory.get_ts; try exact GET2. i. des.
+      { rewrite x1 in *. inv l. }
+      exploit Memory.max_ts_spec; try exact GET2. i. des.
+      exploit TimeFacts.lt_le_lt; try exact x1; try exact MAX0. i.
+      rewrite x3 in l. specialize (TM loc). rewrite l in TM. timetac.
+    - subst. rewrite x2 in *. timetac.
+  Qed.
+
+  Lemma cap_flex_covered
+        mem0 mem1 tm
+        (CAP: cap_flex mem0 mem1 tm)
+        (CLOSED: Memory.closed mem0)
+        (TM: forall loc, Time.lt (Memory.max_ts loc mem0) (tm loc))
+        loc to
+    :
+      Interval.mem (Time.bot, (tm loc)) to
+      <->
+      covered loc to mem1.
+  Proof.
+    split; i.
+    {
+      inv H. inv CAP. set (@cell_elements_least
+                             (mem0 loc)
+                             (fun to' => Time.le to to')). des; cycle 1.
+      { destruct (Time.le_lt_dec to (Memory.max_ts loc mem0)).
+        - exfalso. exploit Memory.max_ts_spec.
+          + eapply CLOSED.
+          + i. des. exploit EMPTY; eauto.
+        - econs.
+          + eapply BACK.
+          + econs; eauto. }
+      set (@cell_elements_greatest
+             (mem0 loc)
+             (fun to' => Time.lt to' to)). des; cycle 1.
+      { exfalso. exploit EMPTY.
+        - eapply CLOSED.
+        - eauto.
+        - ss. }
+      destruct (Time.le_lt_dec to from).
+      - exploit MIDDLE.
+        + econs.
+          * eapply GET0.
+          * eapply GET.
+          * eapply TimeFacts.lt_le_lt; eauto.
+          * i. destruct (Memory.get loc ts mem0) eqn:GET1; auto.
+            exfalso. destruct p.
+            destruct (Time.le_lt_dec to ts).
+            { exploit LEAST; eauto. i.
+              eapply Time.lt_strorder. eapply TimeFacts.le_lt_lt.
+              { eapply x. }
+              eapply TimeFacts.le_lt_lt.
+              { eapply TS2. }
+              { eapply memory_get_ts_strong in GET. des; clarify; ss.
+                exfalso. eapply Time.lt_strorder. eapply TimeFacts.le_lt_lt.
+                - eapply l.
+                - eauto. } }
+            { exploit GREATEST; eauto. i.
+              eapply Time.lt_strorder. eapply TimeFacts.le_lt_lt.
+              { eapply x. }
+              { eauto. } }
+        + eapply TimeFacts.lt_le_lt; eauto.
+        + i. econs; eauto. econs; eauto.
+      - econs.
+        + eapply SOUND. eapply GET.
+        + econs; eauto.
+    }
+    {
+      inv H. apply Memory.max_ts_spec in GET. des.
+      inv ITV. ss. econs; ss.
+      - eapply TimeFacts.le_lt_lt; eauto. apply Time.bot_spec.
+      - etrans; eauto. erewrite <- cap_flex_max_ts; eauto.
+    }
+  Qed.
+
 End CAPFLEX.
 
 
@@ -484,47 +574,55 @@ Section MIDDLE.
   Variable L: Loc.t -> bool.
   Variable times: Loc.t -> list Time.t.
 
+  Lemma sim_memory_max_ts_le F extra mem_src mem_tgt
+        (MEM: sim_memory L times F extra mem_src mem_tgt)
+        (MEMTGT: Memory.closed mem_tgt)
+        loc
+    :
+      Time.le (Memory.max_ts loc mem_tgt) (Memory.max_ts loc mem_src).
+  Proof.
+    hexploit (@Memory.max_ts_spec loc).
+    { inv MEMTGT. eapply INHABITED. } i. des.
+    destruct (Memory.get loc (Memory.max_ts loc mem_tgt) mem_src) as [[from_src msg_src]|] eqn:GETSRC; cycle 1.
+    { exfalso. eapply sim_memory_src_none in GETSRC; eauto. des; clarify. }
+    apply Memory.max_ts_spec in GETSRC. des. auto.
+  Qed.
 
   Lemma sim_memory_max_ts_extra F extra mem_src mem_tgt
         (MEM: sim_memory L times F extra mem_src mem_tgt)
-        (MEMSRC: Memory.closed mem_src)
         (MEMTGT: Memory.closed mem_tgt)
         loc
     :
       Memory.max_ts loc mem_src = Memory.max_ts loc mem_tgt \/
       extra loc (Memory.max_ts loc mem_src) (Memory.max_ts loc mem_tgt).
   Proof.
-    hexploit (@Memory.max_ts_spec loc).
-    { inv MEMTGT. eapply INHABITED. } i. des.
-    destruct (Memory.get loc (Memory.max_ts loc mem_tgt) mem_src) as [[from_src msg_src]|] eqn:GETSRC; cycle 1.
-    { exfalso. eapply sim_memory_src_none in GETSRC; eauto. des; clarify. }
-
-    i. hexploit (@Memory.max_ts_spec loc).
-    { inv MEMTGT. eapply INHABITED. } i. des.
-    destruct (Memory.get loc (Memory.max_ts loc mem_tgt) mem_src) eqn:GETSRC0.
-    { destruct p. dup GETSRC0. dup GET. eapply Memory.max_ts_spec in GETSRC0. des.
-      eapply Memory.max_ts_spec in GET0. des.
-      dup GET1. eapply sim_memory_get_larger in GET2; eauto. des.
-      { clarify. left. apply TimeFacts.antisym.
-        { apply Memory.max_ts_spec in GETTGT. des. auto. }
-        { apply Memory.max_ts_spec in GETSRC1. des. auto. }
-      }
-      { right.
-  Admitted.
-
-  Lemma sim_memory_max_ts_le F extra mem_src mem_tgt
-        (MEM: sim_memory L times F extra mem_src mem_tgt)
-        (MEMSRC: Memory.closed mem_src)
-        (MEMTGT: Memory.closed mem_tgt)
-        loc
-    :
-      Time.le (Memory.max_ts loc mem_tgt) (Memory.max_ts loc mem_src).
-  Proof.
-    hexploit sim_memory_max_ts_extra; eauto. i. des.
-    { rewrite H. refl. }
-    { eapply MEM.(sim_memory_wf) in H. des. left. auto. }
+    hexploit sim_memory_max_ts_le; eauto. intros [TS|[]]; auto.
+    assert (exists from_bot msg_bot, <<GETBOTSRC: Memory.get loc Time.bot mem_src = Some (from_bot, msg_bot)>>).
+    { set (MEM0:=MEM.(sim_memory_contents) loc Time.bot).
+      inv MEMTGT. erewrite INHABITED in MEM0. inv MEM0; eauto. }
+    des. eapply Memory.max_ts_spec in GETBOTSRC. des.
+    dup GET. eapply sim_memory_get_larger in GET; eauto. des.
+    { apply Memory.max_ts_spec in GETTGT. des.
+      left. apply Memory.max_ts_spec in GET. des.
+      apply TimeFacts.antisym; auto.
+      destruct (Memory.get loc (Memory.max_ts loc mem_tgt) mem_src) as [[from_src msg_src]|] eqn:GETSRC; cycle 1.
+      { exfalso. eapply sim_memory_src_none in GETSRC; eauto. des; clarify. }
+      eapply Memory.max_ts_spec in GETSRC; eauto. des. auto.
+    }
+    { hexploit (MEM.(sim_memory_wf) loc from (Memory.max_ts loc mem_src)); eauto. i. des.
+      set (MEM0 := MEM.(sim_memory_contents) loc from). inv MEM0; ss. symmetry in H.
+      right. replace (Memory.max_ts loc mem_tgt) with from; auto.
+      apply Memory.max_ts_spec in H; eauto. des. apply TimeFacts.antisym; auto.
+      destruct (Memory.get loc (Memory.max_ts loc mem_tgt) mem_src) as [[ts msg_src]|] eqn:GETSRC; cycle 1.
+      { exfalso. eapply sim_memory_src_none in GETSRC; eauto. des; clarify. }
+      hexploit memory_get_disjoint_strong.
+      { eapply GETSRC. }
+      { eapply GET0. }
+      i. des; auto.
+      { subst. rewrite H in *. timetac. }
+      { exfalso. eapply Time.lt_strorder. etrans; [apply TS|eauto]. }
+    }
   Qed.
-
 
   (* sim memory strong *)
   Inductive sim_memory_content_strong
@@ -627,6 +725,30 @@ Section MIDDLE.
       inv MEM0; try by (exfalso; eapply NEXTRA0; eauto).
       eapply MEM.(sim_memory_strong_wf) in EXTRA. des.
       apply UNIQUE in EXTRA0. subst. eauto. }
+  Qed.
+
+  Lemma sim_memory_strong_left_end_inv F extra mem_src mem_tgt
+        (MEM: sim_memory_strong F extra mem_src mem_tgt)
+        loc from to_src msg_src
+        (GETSRC: Memory.get loc to_src mem_src = Some (from, msg_src))
+        (NONE: Memory.get loc from mem_src = None)
+    :
+      exists to_tgt msg_tgt,
+        (<<GETTGT: Memory.get loc to_tgt mem_tgt = Some (from, msg_tgt)>>).
+  Proof.
+    set (MEM0:=MEM.(sim_memory_strong_contents) loc to_src).
+    rewrite GETSRC in *. inv MEM0.
+    { des; clarify; eauto.
+      set (MEM0:=MEM.(sim_memory_strong_contents) loc from).
+      inv MEM0; try by (exfalso; eapply NEXTRA0; eauto).
+      rewrite NONE in *. clarify. }
+    { des; clarify; eauto.
+      set (MEM0:=MEM.(sim_memory_strong_contents) loc from).
+      inv MEM0; try by (exfalso; eapply NEXTRA0; eauto).
+      rewrite NONE in *. clarify. }
+    { exploit (MEM.(sim_memory_strong_wf) loc from to_src); eauto. i. des.
+      set (MEM0:=MEM.(sim_memory_strong_contents) loc from). inv MEM0; ss.
+      rewrite NONE in *. clarify. }
   Qed.
 
   Lemma sim_memory_right_end F extra mem_src mem_tgt
@@ -773,14 +895,14 @@ Section MIDDLE.
 
   Lemma cap_left_end mem1 mem2 tm loc ts1 ts2 msg1
         (MEM: Memory.closed mem1)
-        (CAP: cap mem1 mem2)
+        (CAP: cap_flex mem1 mem2 tm)
         (GET: Memory.get loc ts2 mem1 = Some (ts1, msg1))
     :
       exists ts0 msg0,
         (<<GET: Memory.get loc ts1 mem2 = Some (ts0, msg0)>>).
   Proof.
     destruct (Memory.get loc ts1 mem1) as [[ts0 msg0]|] eqn:GETORG.
-    { eapply Memory.cap_le in GETORG; eauto. refl. }
+    { inv CAP. eapply SOUND in GETORG; eauto. }
     { hexploit (@cell_elements_greatest
                   (mem1 loc)
                   (fun ts => Time.lt ts ts1)). i. des; cycle 1.
@@ -807,23 +929,22 @@ Section MIDDLE.
     }
   Qed.
 
-  Lemma sim_memory_strong_cap F extra mem_src mem_tgt cap_src cap_tgt
+  Lemma sim_memory_strong_cap F extra mem_src mem_tgt tm cap_src cap_tgt
         (MEM: sim_memory_strong F extra mem_src mem_tgt)
         (MEMSRC: Memory.closed mem_src)
         (MEMTGT: Memory.closed mem_tgt)
         (MEMWF: memory_times_wf times mem_tgt)
-        (CAPSRC: Memory.cap mem_src cap_src)
-        (CAPTGT: cap_flex mem_tgt cap_tgt (Memory.max_timemap cap_src))
+        (CAPSRC: cap_flex mem_src cap_src tm)
+        (CAPTGT: cap_flex mem_tgt cap_tgt tm)
+        (TM: forall loc, Time.lt (Memory.max_ts loc mem_src) (tm loc))
     :
       sim_memory L times F extra cap_src cap_tgt.
   Proof.
-    assert (NEXMAX: forall loc, Time.lt (Memory.max_ts loc mem_tgt) (Memory.max_timemap cap_src loc)).
-    { i. unfold Memory.max_timemap. erewrite (@Memory.cap_max_ts mem_src cap_src); eauto.
-      eapply TimeFacts.le_lt_lt.
-      { eapply sim_memory_max_ts_le; try apply MEMSRC; eauto.
-        eapply sim_memory_strong_sim_memory; eauto. }
-      { eapply Time.incr_spec. }
-    }
+    assert (TMTGT: forall loc, Time.lt (Memory.max_ts loc mem_tgt) (tm loc)).
+    { i. eapply TimeFacts.le_lt_lt; eauto.
+      eapply sim_memory_max_ts_le; try apply MEMSRC; eauto.
+      eapply sim_memory_strong_sim_memory; eauto. }
+
     dup CAPTGT. inv CAPTGT0. dup CAPSRC. inv CAPSRC0. econs.
     { i. set (MEM0:=MEM.(sim_memory_strong_contents) loc ts).
       inv MEM0; symmetry in H; symmetry in H0; rename H into GETMEMTGT; rename H0 into GETMEMSRC.
@@ -831,13 +952,10 @@ Section MIDDLE.
         { eapply cap_flex_inv in GETTGT; try apply CAPTGT; eauto. des; clarify.
           { hexploit sim_memory_strong_adjancent; eauto. i. des.
             erewrite MIDDLE0; eauto. }
-          { revert NEXTRA NPROM. unfold Memory.max_timemap.
-            erewrite Memory.cap_max_ts; try apply CAPSRC; eauto.
-            erewrite BACK0. i. econs 2; auto.
+          { erewrite BACK0. i. econs 2; auto.
             { eapply sim_memory_max_ts_le; eauto. eapply sim_memory_strong_sim_memory; eauto. }
             { i. hexploit sim_memory_max_ts_extra.
               { eapply sim_memory_strong_sim_memory; eauto. }
-              { eauto. }
               { eauto. }
               i. des.
               { rewrite H. apply eq_lb_time. }
@@ -858,28 +976,17 @@ Section MIDDLE.
           }
         }
         { destruct (Memory.get loc ts cap_src) as [[from_src msg_src]|] eqn:GETSRC; eauto.
-          eapply Memory.cap_inv in GETSRC; try apply CAPSRC; eauto. des; clarify.
-          { inv GETSRC0. eapply
-
-            eapply cap_left_end in GET2; eauto. des.
-
-            cap_left_end
-
-            Memory.adjacent
-
-
-            admit. }
-          { erewrite <- (@Memory.cap_max_ts mem_src cap_src) in GETTGT; eauto.
-            unfold Memory.max_timemap in BACK. erewrite BACK in *. clarify. }
+          eapply cap_flex_inv in GETSRC; try apply CAPSRC; eauto. des; clarify.
+          { inv GETSRC0. exploit sim_memory_strong_left_end_inv; eauto. i. des.
+            eapply cap_left_end in GETTGT0; eauto. des. clarify. }
+          { erewrite BACK in GETTGT. clarify. }
+        }
       }
-      { eapply Memory.cap_le in GETMEMSRC; [|try apply CAPSRC|refl].
-        eapply SOUND in GETMEMTGT.
+      { eapply SOUND0 in GETMEMSRC. eapply SOUND in GETMEMTGT.
         rewrite GETMEMSRC. rewrite GETMEMTGT. eauto. }
-      { eapply Memory.cap_le in GETMEMSRC; [|try apply CAPSRC|refl].
-        eapply SOUND in GETMEMTGT.
+      { eapply SOUND0 in GETMEMSRC. eapply SOUND in GETMEMTGT.
         rewrite GETMEMSRC. rewrite GETMEMTGT. eauto. }
-      { dup GETMEMSRC. eapply Memory.cap_le in GETMEMSRC; [|try apply CAPSRC|refl].
-        rewrite GETMEMSRC.
+      { dup GETMEMSRC. eapply SOUND0 in GETMEMSRC. rewrite GETMEMSRC.
         destruct (Memory.get loc ts cap_tgt) as [[from_tgt msg_tgt]|] eqn:GETTGT; eauto.
         eapply cap_flex_inv in GETTGT; eauto. des; clarify.
         { inv GETTGT0. eapply MEM.(sim_memory_strong_wf) in EXTRA. des.
@@ -888,1079 +995,14 @@ Section MIDDLE.
           { auto. }
           i. timetac.
         }
-        { exfalso. unfold Memory.max_timemap in GETMEMSRC0.
-          erewrite Memory.cap_max_ts in GETMEMSRC0; try apply CAPSRC; eauto.
-          apply Memory.max_ts_spec in GETMEMSRC0. des.
-          eapply Time.lt_strorder. eapply TimeFacts.lt_le_lt.
-          { eapply Time.incr_spec. }
+        { eapply Memory.max_ts_spec in GETMEMSRC0. des.
+          exfalso. eapply Time.lt_strorder. eapply TimeFacts.lt_le_lt.
+          { eapply TM. }
           { eapply MAX. }
         }
       }
     }
     { eapply MEM.(sim_memory_strong_wf); eauto. }
   Qed.
-
-
-  Lemma sim_memory_strong_cap F extra mem_src mem_tgt cap_src cap_tgt
-        (MEM: sim_memory_strong F extra mem_src mem_tgt)
-        (MEMSRC: Memory.closed mem_src)
-        (MEMTGT: Memory.closed mem_tgt)
-        (CAPSRC: Memory.cap mem_src cap_src)
-        (CAPTGT: cap_flex mem_tgt cap_tgt (Memory.max_timemap cap_src))
-    :
-      sim_memory L times F extra cap_src cap_tgt.
-  Proof.
-    assert (NEXMAX: forall loc, Time.lt (Memory.max_ts loc mem_tgt) (Memory.max_timemap cap_src loc)).
-    { i. unfold Memory.max_timemap. erewrite (@Memory.cap_max_ts mem_src cap_src); eauto.
-      eapply TimeFacts.le_lt_lt.
-      { eapply sim_memory_max_ts; eauto. eapply sim_memory_strong_sim_memory; eauto. }
-      { eapply Time.incr_spec. }
-    }
-    dup CAPTGT. inv CAPTGT0. econs.
-    { i. set (MEM0:=MEM.(sim_memory_strong_contents) loc ts).
-      inv MEM0; symmetry in H; symmetry in H0; rename H into GETMEMTGT; rename H0 into GETMEMSRC.
-      {
-
-
-        admit. }
-      { eapply Memory.cap_le in GETMEMSRC; [|try apply CAPSRC|refl].
-        eapply SOUND in GETMEMTGT.
-        rewrite GETMEMSRC. rewrite GETMEMTGT. eauto. }
-      { eapply Memory.cap_le in GETMEMSRC; [|try apply CAPSRC|refl].
-        eapply SOUND in GETMEMTGT.
-        rewrite GETMEMSRC. rewrite GETMEMTGT. eauto. }
-       memor{
-        dup GETMEMSRC. eapply Memory.cap_le in GETMEMSRC; [|try apply CAPSRC|refl].
-        rewrite GETMEMSRC.
-        destruct (Memory.get loc ts cap_tgt) as [[from_tgt msg_tgt]|] eqn:GETTGT; eauto.
-        eapply cap_flex_inv in GETTGT; eauto. des; clarify.
-        { inv GETTGT0.
-
-
-          admit. }
-        {
-
-          admit. }
-      }
-    }
-    { eapply MEM.(sim_memory_strong_wf); eauto. }
-  Qed.
-
-      i. eapp
-
-      Memory.cap_inv
-
-
-
-        others self extra_others extra_self
-        prom_src prom_tgt mem_src mem_tgt
-        (MEM: sim_memory_strong (others \\2// self) (extra_others \\3// extra_self) mem_src mem_tgt)
-        (MLETGT: Memory.le prom_tgt mem_tgt)
-        (MLESRC: Memory.le prom_src mem_src)
-        (FIN: Memory.finite prom_src)
-        (BOTNONESRC: Memory.bot_none prom_src)
-        (PROM: sim_promise self extra_self prom_src prom_tgt)
-        (MEMWF: memory_times_wf times mem_tgt)
-    :
-      exists prom_src' mem_src',
-        (<<FUTURE: reserve_future_memory prom_src mem_src prom_src' mem_src'>>) /\
-        (<<MEM: sim_memory (others \\2// self) (extra_others \\3// extra_self) mem_src' mem_tgt>>) /\
-        (<<PROM: sim_promise_strong
-                   self extra_self (extra_others \\3// extra_self)
-                   prom_src' prom_tgt>>).
-  Proof.
-    exploit sim_promise_weak_list_exists; eauto. i. des.
-    clear PROM. ginduction l.
-    { i. exists prom_src, mem_src. splits; auto.
-      eapply sim_promise_list_nil; eauto. }
-    i. destruct a as [loc ts].
-
-
-  Lemma sim_promise_weak_stengthen others self extra_others extra_self
-        prom_src prom_tgt mem_src mem_tgt
-        (MEM: sim_memory (others \\2// self) (extra_others \\3// extra_self) mem_src mem_tgt)
-        (MLETGT: Memory.le prom_tgt mem_tgt)
-        (MLESRC: Memory.le prom_src mem_src)
-        (FIN: Memory.finite prom_src)
-        (BOTNONESRC: Memory.bot_none prom_src)
-        (PROM: sim_promise self extra_self prom_src prom_tgt)
-        (MEMWF: memory_times_wf times mem_tgt)
-    :
-      exists prom_src' mem_src',
-        (<<FUTURE: reserve_future_memory prom_src mem_src prom_src' mem_src'>>) /\
-        (<<MEM: sim_memory (others \\2// self) (extra_others \\3// extra_self) mem_src' mem_tgt>>) /\
-        (<<PROM: sim_promise_strong
-                   self extra_self (extra_others \\3// extra_self)
-                   prom_src' prom_tgt>>).
-  Proof.
-    exploit sim_promise_weak_list_exists; eauto. i. des.
-    clear PROM. ginduction l.
-    { i. exists prom_src, mem_src. splits; auto.
-      eapply sim_promise_list_nil; eauto. }
-    i. destruct a as [loc ts].
-
-
-  Lemma sim_memory_content_strong
-
-
-
-  Lemma sim_promise_content_strong_sim_promise_content
-        loc ts F extra get0 get1 extra_all
-        (SIM: sim_promise_content_strong F extra extra_all loc ts  get0 get1)
-    :
-      sim_promise_content F extra loc ts get0 get1.
-  Proof.
-    inv SIM; econs; eauto.
-  Qed.
-
-  Record sim_promise_strong
-         (self: Loc.t -> Time.t -> Prop)
-         (extra: Loc.t -> Time.t -> Time.t -> Prop)
-         (extra_all: Loc.t -> Time.t -> Time.t -> Prop)
-         (prom_src prom_tgt: Memory.t): Prop :=
-    {
-      sim_promise_strong_contents:
-        forall loc ts,
-          sim_promise_content_strong (self loc ts) (extra loc ts) (extra_all loc)
-                                     loc ts
-                                     (Memory.get loc ts prom_src)
-                                     (Memory.get loc ts prom_tgt);
-      sim_promise_strong_wf:
-        forall loc from ts (EXTRA: extra loc ts from),
-          (<<FORGET: self loc from>>) /\
-          (<<LB: lb_time (times loc) from ts>>) /\
-          (<<TS: Time.lt from ts>>);
-      sim_promise_strong_extra:
-        forall loc ts (SELF: self loc ts),
-        exists to,
-          (<<GET: Memory.get loc to prom_src = Some (ts, Message.reserve)>>) /\
-          (<<TS: Time.lt ts to>>);
-    }.
-
-  Lemma sim_promise_strong_sim_promise
-        self extra extra_all prom_src prom_tgt
-        (SIM: sim_promise_strong self extra extra_all prom_src prom_tgt)
-    :
-      sim_promise self extra prom_src prom_tgt.
-  Proof.
-    econs.
-    - ii. eapply sim_promise_content_strong_sim_promise_content; eauto.
-      eapply SIM; eauto.
-    - apply SIM.
-    - apply SIM.
-  Qed.
-
-  Record sim_promise_list
-         (self: Loc.t -> Time.t -> Prop)
-         (extra: Loc.t -> Time.t -> Time.t -> Prop)
-         (extra_all: Loc.t -> Time.t -> Time.t -> Prop)
-         (prom_src prom_tgt: Memory.t)
-         (l: list (Loc.t * Time.t)): Prop :=
-    {
-      sim_promise_list_contents:
-        forall loc ts,
-          (<<NORMAL: sim_promise_content_strong (self loc ts) (extra loc ts) (extra_all loc) loc ts
-                                                (Memory.get loc ts prom_src)
-                                                (Memory.get loc ts prom_tgt)>>) \/
-          ((<<LIN: List.In (loc, ts) l>>) /\
-           (<<WEAK: sim_promise_content (self loc ts) (extra loc ts) loc ts
-                                        (Memory.get loc ts prom_src)
-                                        (Memory.get loc ts prom_tgt)>>));
-      sim_promise_list_wf:
-        forall loc from ts (EXTRA: extra loc ts from),
-          (<<FORGET: self loc from>>) /\
-          (<<LB: lb_time (times loc) from ts>>) /\
-          (<<TS: Time.lt from ts>>);
-      sim_promise_list_extra:
-        forall loc ts (SELF: self loc ts),
-        exists to,
-          (<<GET: Memory.get loc to prom_src = Some (ts, Message.reserve)>>) /\
-          (<<TS: Time.lt ts to>>);
-    }.
-
-  Lemma sim_promise_list_nil self extra extra_all prom_src prom_tgt
-        (SIM: sim_promise_list self extra extra_all prom_src prom_tgt [])
-    :
-      sim_promise_strong self extra extra_all prom_src prom_tgt.
-  Proof.
-    econs.
-    - ii. hexploit SIM.(sim_promise_list_contents); eauto. i. des; eauto. ss.
-    - apply SIM.
-    - apply SIM.
-  Qed.
-
-  Lemma sim_promise_weak_list_exists self extra extra_all prom_src prom_tgt
-        (SIM: sim_promise self extra prom_src prom_tgt)
-        (FIN: Memory.finite prom_src)
-    :
-      exists l,
-        (<<SIM: sim_promise_list self extra extra_all prom_src prom_tgt l>>).
-  Proof.
-    unfold Memory.finite in *. des.
-    hexploit (@list_filter_exists
-                (Loc.t * Time.t)
-                (fun locts =>
-                   let (loc, ts) := locts in
-                   ~ sim_promise_content_strong (self loc ts) (extra loc ts) (extra_all loc) loc ts
-                     (Memory.get loc ts prom_src)
-                     (Memory.get loc ts prom_tgt))
-                dom).
-    i. des. exists l'. econs; [|apply SIM|apply SIM].
-    ii. set (PROM:= SIM.(sim_promise_contents) loc ts).
-    destruct (classic (List.In (loc,ts) l')).
-    - right. splits; auto.
-    - left. red. inv PROM; try by (econs; eauto).
-      + apply NNPP. ii. exploit FIN; eauto. i.
-        hexploit (proj1 (@COMPLETE (loc, ts))); auto.
-        splits; auto. ii. rewrite H1 in *. rewrite H2 in *. auto.
-      + apply NNPP. ii. exploit FIN; eauto. i.
-        hexploit (proj1 (@COMPLETE (loc, ts))); auto.
-        splits; auto. ii. rewrite H1 in *. rewrite H2 in *. auto.
-  Qed.
-
-  Lemma sim_promise_weak_stengthen others self extra_others extra_self
-        prom_src prom_tgt mem_src mem_tgt
-        (MEM: sim_memory (others \\2// self) (extra_others \\3// extra_self) mem_src mem_tgt)
-        (MLETGT: Memory.le prom_tgt mem_tgt)
-        (MLESRC: Memory.le prom_src mem_src)
-        (FIN: Memory.finite prom_src)
-        (BOTNONESRC: Memory.bot_none prom_src)
-        (PROM: sim_promise self extra_self prom_src prom_tgt)
-        (MEMWF: memory_times_wf times mem_tgt)
-    :
-      exists prom_src' mem_src',
-        (<<FUTURE: reserve_future_memory prom_src mem_src prom_src' mem_src'>>) /\
-        (<<MEM: sim_memory (others \\2// self) (extra_others \\3// extra_self) mem_src' mem_tgt>>) /\
-        (<<PROM: sim_promise_strong
-                   self extra_self (extra_others \\3// extra_self)
-                   prom_src' prom_tgt>>).
-  Proof.
-    exploit sim_promise_weak_list_exists; eauto. i. des.
-    clear PROM. ginduction l.
-    { i. exists prom_src, mem_src. splits; auto.
-      eapply sim_promise_list_nil; eauto. }
-    i. destruct a as [loc ts].
-
-    cut (sim_promise_content_strong (self loc ts) (extra_self loc ts)
-                                    ((extra_others \\3// extra_self) loc)
-                                    loc ts
-                                    (Memory.get loc ts prom_src)
-                                    (Memory.get loc ts prom_tgt) \/
-         exists prom_src' mem_src',
-           (<<FUTURE: reserve_future_memory prom_src mem_src prom_src' mem_src'>>) /\
-           (<<MEM: sim_memory (others \\2// self) (extra_others \\3// extra_self) mem_src' mem_tgt>>) /\
-           (<<PROM: sim_promise_list
-                      self extra_self (extra_others \\3// extra_self)
-                      prom_src' prom_tgt l>>)).
-    { intros H. match goal with
-                | [H:?A \/ ?B |- _ ] => cut B
-                end.
-      { clear H. i. des. exploit IHl.
-        { eapply MEM0. }
-        { eauto. }
-        { eapply reserve_future_memory_le; eauto. }
-        { eapply reserve_future_memory_finite; eauto. }
-        { eapply reserve_future_memory_bot_none; try apply BOTNONESRC; eauto. }
-        { eauto. }
-        { eauto. }
-        i. des. exists prom_src'0, mem_src'0. splits; eauto.
-        eapply reserve_future_memory_trans; eauto. }
-      { des; eauto. exists prom_src, mem_src. splits; auto.
-        econs; [|apply SIM|apply SIM]. ii.
-        set (PROM:=SIM.(sim_promise_list_contents) loc0 ts0).
-        ss. des; clarify; auto. }
-    }
-
-    set (SIM0:= SIM.(sim_promise_list_contents) loc ts). des; auto.
-    inv WEAK.
-    { left. econs 1; eauto. }
-    { left. econs 2; eauto. }
-    { clear LIN. symmetry in H. symmetry in H0.
-      rename H into PROMTGT. rename H0 into PROMSRC.
-      dup PROMSRC. dup PROMTGT. apply MLESRC in PROMSRC0. apply MLETGT in PROMTGT0.
-      rename PROMSRC0 into MEMSRC. rename PROMTGT0 into MEMTGT.
-      set (MEM0:=MEM.(sim_memory_contents) loc ts).
-      rewrite MEMSRC in MEM0. rewrite MEMTGT in MEM0. inv MEM0; ss.
-      destruct (classic (self loc from_src)) as [SELF|NSELF].
-      { left. exploit sim_memory_from_forget; eauto. ss. right. auto. }
-
-      hexploit (@Memory.remove_exists prom_src); eauto.
-      intros [prom_src' REMOVEPROM].
-      hexploit (@Memory.remove_exists_le prom_src mem_src); eauto.
-      intros [mem_src' REMOVEMEM].
-      assert (REMOVE: Memory.promise prom_src mem_src loc from_src ts Message.reserve prom_src' mem_src' Memory.op_kind_cancel).
-      { econs; eauto. }
-      destruct (classic (exists from_src', (extra_others \\3// extra_self) loc from_src' from_tgt))
-        as [[from_src' EXTRA]|].
-      { guardH EXTRA.
-        hexploit (@Memory.add_exists mem_src' loc from_src' ts Message.reserve).
-        { ii. erewrite Memory.remove_o in GET2; eauto. des_ifs. guardH o.
-          hexploit sim_memory_disjoint.
-          { eauto. }
-          { eauto. }
-          { apply MEMTGT. }
-          { eapply GET2. }
-          { instantiate (1:=x). inv LHS. econs; ss.
-            transitivity from_src'; auto.
-            eapply MEM.(sim_memory_wf) in EXTRA. des; auto. }
-          { eauto. }
-          i. destruct H as [EQ|[EQ [FORGET [EXTRA0 TS]]]].
-          { des; subst. destruct o; ss. }
-          { guardH FORGET. guardH EXTRA0.
-            hexploit sim_memory_extra_inj.
-            { eapply MEM. }
-            { eapply EXTRA0. }
-            { eapply EXTRA. }
-            i. subst. inv LHS. inv RHS. ss. timetac. }
-        }
-        { eapply MEM.(sim_memory_wf) in EXTRA. destruct EXTRA as [_ EXTRA]. des.
-          eapply LB0.
-          { eapply MEMWF in MEMTGT. des; auto. }
-          { apply memory_get_ts_strong in MEMTGT. des; auto.
-            subst. erewrite BOTNONESRC in PROMSRC. clarify. }
-        }
-        { econs; eauto. }
-        intros [mem_src'' ADDMEM].
-        hexploit (@Memory.add_exists_le prom_src' mem_src'); eauto.
-        { eapply promise_memory_le; eauto. }
-        intros [prom_src'' ADDPROM].
-        assert (ADD: Memory.promise prom_src' mem_src' loc from_src' ts Message.reserve prom_src'' mem_src'' Memory.op_kind_add).
-        { econs; eauto. i. clarify. }
-        right. exists prom_src'', mem_src''. splits; eauto.
-        { econs; [|apply MEM]. i.
-          erewrite (@Memory.add_o mem_src''); eauto.
-          erewrite (@Memory.remove_o mem_src'); eauto. des_ifs.
-          { ss. des; subst. rewrite MEMTGT. econs; eauto.
-            { left. eapply sim_memory_wf; eauto. ss. eauto. }
-            { i. apply MEM.(sim_memory_wf). ss. }
-            { i. ss. }
-          }
-          { apply MEM. }
-        }
-        { econs; [|apply SIM|].
-          { i. erewrite (@Memory.add_o prom_src''); eauto.
-            erewrite (@Memory.remove_o prom_src'); eauto. des_ifs.
-            { ss. des; subst. left. rewrite PROMTGT. econs; eauto. }
-            { guardH o. set (PROM:=SIM.(sim_promise_list_contents) loc0 ts0).
-              des; auto. right. splits; eauto. ss. des; auto.
-              clarify. unguard. des; ss. }
-          }
-          { i. set (PROM:=SIM.(sim_promise_list_extra) loc0 ts0 SELF).
-            des. exists to.
-            erewrite Memory.add_o; eauto. erewrite Memory.remove_o; eauto. des_ifs.
-            ss. des; subst. clarify. }
-        }
-      }
-
-      { hexploit (@Memory.add_exists mem_src' loc from_tgt ts Message.reserve).
-        { ii. erewrite Memory.remove_o in GET2; eauto. des_ifs. guardH o.
-          hexploit sim_memory_disjoint.
-          { eauto. }
-          { eauto. }
-          { eapply MEMTGT. }
-          { eapply GET2. }
-          { instantiate (1:=x). eauto. }
-          { eauto. }
-          i. destruct H0 as [EQ|[EQ [FORGET [EXTRA TS]]]].
-          { des; subst. destruct o; ss. }
-          { guardH FORGET. guardH EXTRA.
-            eapply H. esplits; eauto. }
-        }
-        { apply memory_get_ts_strong in MEMTGT. des; auto. subst.
-          erewrite BOTNONESRC in PROMSRC. clarify. }
-        { econs. }
-        intros [mem_src'' ADDMEM].
-        hexploit (@Memory.add_exists_le prom_src' mem_src'); eauto.
-        { eapply promise_memory_le; eauto. }
-        intros [prom_src'' ADDPROM].
-        assert (ADD: Memory.promise prom_src' mem_src' loc from_tgt ts Message.reserve prom_src'' mem_src'' Memory.op_kind_add).
-        { econs; eauto. i. clarify. }
-        right. exists prom_src'', mem_src''. splits; eauto.
-        { econs; [|apply MEM]. i.
-          erewrite (@Memory.add_o mem_src''); eauto.
-          erewrite (@Memory.remove_o mem_src'); eauto. des_ifs.
-          { ss. des; subst. rewrite MEMTGT. econs; eauto.
-            { refl. }
-            { i. apply eq_lb_time. }
-          }
-          { apply MEM. }
-        }
-        { econs; [|apply SIM|].
-          { i. erewrite (@Memory.add_o prom_src''); eauto.
-            erewrite (@Memory.remove_o prom_src'); eauto. des_ifs.
-            { ss. des; subst. left. rewrite PROMTGT. eauto. }
-            { guardH o. set (PROM:=SIM.(sim_promise_list_contents) loc0 ts0).
-              des; auto. right. splits; eauto. ss. des; auto.
-              clarify. unguard. des; ss. }
-          }
-          { i. set (PROM:=SIM.(sim_promise_list_extra) loc0 ts0 SELF).
-            des. exists to.
-            erewrite Memory.add_o; eauto. erewrite Memory.remove_o; eauto. des_ifs.
-            ss. des; subst. clarify. }
-        }
-      }
-    }
-
-    { clear LIN. symmetry in H. symmetry in H0.
-      rename H into PROMTGT. rename H0 into PROMSRC.
-      dup PROMSRC. dup PROMTGT. apply MLESRC in PROMSRC0. apply MLETGT in PROMTGT0.
-      rename PROMSRC0 into MEMSRC. rename PROMTGT0 into MEMTGT.
-      set (MEM0:=MEM.(sim_memory_contents) loc ts).
-      rewrite MEMSRC in MEM0. rewrite MEMTGT in MEM0. inv MEM0; ss. guardH PROM0.
-      destruct (classic (self loc from_src)) as [SELF|NSELF].
-      { left. exploit sim_memory_from_forget; eauto. ss. right. auto. }
-
-      hexploit (@Memory.remove_exists prom_src); eauto.
-      intros [prom_src' REMOVEPROM].
-      hexploit (@Memory.remove_exists_le prom_src mem_src); eauto.
-      intros [mem_src' REMOVEMEM].
-      assert (REMOVE: Memory.promise prom_src mem_src loc from_src ts Message.reserve prom_src' mem_src' Memory.op_kind_cancel).
-      { econs; eauto. }
-      destruct (classic (exists from_src', (extra_others \\3// extra_self) loc from_src' from_tgt))
-        as [[from_src' EXTRA]|].
-      { guardH EXTRA.
-        hexploit (@Memory.add_exists mem_src' loc from_src' ts Message.reserve).
-        { ii. erewrite Memory.remove_o in GET2; eauto. des_ifs. guardH o.
-          hexploit sim_memory_disjoint.
-          { eauto. }
-          { eauto. }
-          { eapply MEMTGT. }
-          { eapply GET2. }
-          { instantiate (1:=x). inv LHS. econs; ss.
-            transitivity from_src'; auto.
-            eapply MEM.(sim_memory_wf) in EXTRA. des; auto. }
-          { eauto. }
-          i. destruct H as [EQ|[EQ [FORGET [EXTRA0 TS]]]].
-          { des; subst. destruct o; ss. }
-          { guardH FORGET. guardH EXTRA0.
-            hexploit sim_memory_extra_inj.
-            { eapply MEM. }
-            { eapply EXTRA0. }
-            { eapply EXTRA. }
-            i. subst. inv LHS. inv RHS. ss. timetac. }
-        }
-        { eapply MEM.(sim_memory_wf) in EXTRA. destruct EXTRA as [_ EXTRA]. des.
-          eapply LB0.
-          { eapply MEMWF in MEMTGT. des; auto. }
-          { apply memory_get_ts_strong in MEMTGT. des; auto.
-            subst. erewrite BOTNONESRC in PROMSRC. clarify. }
-        }
-        { econs; eauto. }
-        intros [mem_src'' ADDMEM].
-        hexploit (@Memory.add_exists_le prom_src' mem_src'); eauto.
-        { eapply promise_memory_le; eauto. }
-        intros [prom_src'' ADDPROM].
-        assert (ADD: Memory.promise prom_src' mem_src' loc from_src' ts Message.reserve prom_src'' mem_src'' Memory.op_kind_add).
-        { econs; eauto. i. clarify. }
-        right. exists prom_src'', mem_src''. splits; eauto.
-        { econs; [|apply MEM]. i.
-          erewrite (@Memory.add_o mem_src''); eauto.
-          erewrite (@Memory.remove_o mem_src'); eauto. des_ifs.
-          { ss. des; subst. rewrite MEMTGT.
-            econs; eauto.
-            { left. eapply sim_memory_wf; eauto. ss. eauto. }
-            { i. apply MEM.(sim_memory_wf). ss. }
-          }
-          { apply MEM. }
-        }
-        { econs; [|apply SIM|].
-          { i. erewrite (@Memory.add_o prom_src''); eauto.
-            erewrite (@Memory.remove_o prom_src'); eauto. des_ifs.
-            { ss. des; subst. left. rewrite PROMTGT. econs; eauto. }
-            { guardH o. set (PROM1:=SIM.(sim_promise_list_contents) loc0 ts0).
-              des; auto. right. splits; eauto. ss. des; auto.
-              clarify. unguard. des; ss. }
-          }
-          { i. set (PROM1:=SIM.(sim_promise_list_extra) loc0 ts0 SELF).
-            des. exists to.
-            erewrite Memory.add_o; eauto. erewrite Memory.remove_o; eauto. des_ifs.
-            ss. des; subst. clarify. }
-        }
-      }
-
-      { hexploit (@Memory.add_exists mem_src' loc from_tgt ts Message.reserve).
-        { ii. erewrite Memory.remove_o in GET2; eauto. des_ifs. guardH o.
-          hexploit sim_memory_disjoint.
-          { eauto. }
-          { eauto. }
-          { eapply MEMTGT. }
-          { eapply GET2. }
-          { instantiate (1:=x). eauto. }
-          { eauto. }
-          i. destruct H0 as [EQ|[EQ [FORGET [EXTRA TS]]]].
-          { des; subst. destruct o; ss. }
-          { guardH FORGET. guardH EXTRA.
-            eapply H. esplits; eauto. }
-        }
-        { apply memory_get_ts_strong in MEMTGT. des; auto. subst.
-          erewrite BOTNONESRC in PROMSRC. clarify. }
-        { econs. }
-        intros [mem_src'' ADDMEM].
-        hexploit (@Memory.add_exists_le prom_src' mem_src'); eauto.
-        { eapply promise_memory_le; eauto. }
-        intros [prom_src'' ADDPROM].
-        assert (ADD: Memory.promise prom_src' mem_src' loc from_tgt ts Message.reserve prom_src'' mem_src'' Memory.op_kind_add).
-        { econs; eauto. i. clarify. }
-        right. exists prom_src'', mem_src''. splits; eauto.
-        { econs; [|apply MEM]. i.
-          erewrite (@Memory.add_o mem_src''); eauto.
-          erewrite (@Memory.remove_o mem_src'); eauto. des_ifs.
-          { ss. des; subst. rewrite MEMTGT.
-            econs; eauto.
-            { refl. }
-            { apply eq_lb_time. }
-          }
-          { apply MEM. }
-        }
-        { econs; [|apply SIM|].
-          { i. erewrite (@Memory.add_o prom_src''); eauto.
-            erewrite (@Memory.remove_o prom_src'); eauto. des_ifs.
-            { ss. des; subst. left. rewrite PROMTGT. eauto. }
-            { guardH o. set (PROM1:=SIM.(sim_promise_list_contents) loc0 ts0).
-              des; auto. right. splits; eauto. ss. des; auto.
-              clarify. unguard. des; ss. }
-          }
-          { i. set (PROM1:=SIM.(sim_promise_list_extra) loc0 ts0 SELF).
-            des. exists to.
-            erewrite Memory.add_o; eauto. erewrite Memory.remove_o; eauto. des_ifs.
-            ss. des; subst. clarify. }
-        }
-      }
-    }
-    { left. econs 5; eauto. }
-  Qed.
-
-
-  Definition promises_list
-             (prom_src prom_tgt: Memory.t)
-             (others: Loc.t -> Time.t -> Prop)
-             (self: Loc.t -> Time.t -> Prop)
-             (extra_self: Loc.t -> Time.t -> Prop)
-
-             (l: list (Loc
-
-  Inductive
-
-  sim_promise_strong
-
-  Induct
-
-  Inductive mid_memory (mem_src mem_tgt: Memory.t)
-
-
-  Lemma mid
-
-  Lemma middle_state_exists
-        others self lc_src lc_tgt sc mem_src mem_tgt
-        (views: Loc.t -> Time.t -> list View.t)
-        times
-        (MEM: sim_memory L (others \2/ self) mem_src mem_tgt)
-        (SCSRC: Memory.closed_timemap sc mem_src)
-        (SCTGT: Memory.closed_timemap sc mem_tgt)
-        (MEMSRC: Memory.closed mem_src)
-        (MEMTGT: Memory.closed mem_tgt)
-        (LOCALSRC: Local.wf lc_src mem_src)
-        (LOCALTGT: Local.wf lc_tgt mem_tgt)
-        (SIM: sim_local L self lc_src lc_tgt)
-        (EXCLUSIVE: forall loc' ts' (OTHER: others loc' ts'),
-            exists from msg, <<UNCH: unchangable mem_src lc_src.(Local.promises) loc' ts' from msg>>)
-        (JOINED: forall loc ts (NLOC: ~ L loc), List.Forall (fun vw => Memory.closed_view vw mem_src) (views loc ts))
-
-        cap_src cap_tgt max_src max_tgt
-        (CAPSRC: Memory.cap mem_src cap_src)
-        (CAPTGT: Memory.cap mem_src cap_src)
-        (MAXSRC: Memory.max_concrete_timemap cap_src max_src)
-        (MAXTGT: Memory.max_concrete_timemap cap_tgt max_tgt)
-    :
-      exists f prom_src' cap_src' max_mid
-             lc_mid cap_mid self'
-      ,
-        (<<FUTURE: reserve_future_memory lc_src.(Local.promises) cap_src prom_src' cap_src'>>) /\
-
-        (<<SCMID: Memory.closed_timemap max_src cap_mid>>) /\
-        (<<MEMMID: Memory.closed cap_mid>>) /\
-        (<<LOCALMID: Local.wf lc_mid cap_mid>>) /\
-
-        (<<COMPLETE: forall loc to (IN: List.In (loc, to) times), mappable_time f loc to>>) /\
-
-        (<<MEMORYMAP: memory_map f cap_tgt cap_mid>>) /\
-        (<<LOCALMAP: local_map f lc_tgt lc_mid>>) /\
-        (<<SCMAP: timemap_map f max_tgt max_mid>>) /\
-        (<<SCLE: TimeMap.le max_src max_mid>>) /\
-
-        (<<MEM: sim_memory L (others \2/ self') cap_src' cap_mid>>) /\
-        (<<SIM: sim_local L self' (Local.mk lc_src.(Local.tview) cap_src) lc_mid>>) /\
-
-        (<<PROMATTACH: promises_not_attached self' (promised prom_src') cap_src'>>) /\
-        (<<EXCLUSIVE: forall loc' ts' (OTHER: others loc' ts'),
-            exists from msg, (<<UNCH: unchangable cap_src prom_src' loc' ts' from msg>>)>>) /\
-        (<<JOINED: forall loc ts (NLOC: ~ L loc), List.Forall (fun vw => Memory.closed_view vw cap_src') (views loc ts)>>).
-  Proof.
-  Admitted.
-
-  Record deattached_memory
-         (f: Loc.t -> Time.t -> Time.t -> Prop)
-         (mem mem_d: Memory.t): Prop :=
-    {
-      deattached_memory_get_normal:
-        forall loc to
-               (NMAP0: forall fto, ~ f loc to fto)
-               (NMAP1: forall f_1to, ~ f loc f_1to to),
-          Memory.get loc to mem = Memory.get loc to mem_d;
-      deattached_memory_get_new:
-        forall loc to fto
-               (MAP: f loc to fto),
-        exists from,
-          (<<GETORIG: Memory.get loc to mem = Some (from, Message.reserve)>>) /\
-          (<<GETDNEW: Memory.get loc fto mem_d = Some (from, Message.reserve)>>) /\
-          (<<GETDORIG: Memory.get loc to mem_d = None>>) /\
-          (<<TS0: Time.lt from fto>>) /\
-          (<<TS1: Time.lt fto to>>);
-    }.
-
-  Lemma deattached_memory_map_eq
-        f mem mem_d
-        (DEATTACH: deattached_memory f mem mem_d)
-        loc to fto0 fto1
-        (MAP0: f loc to fto0)
-        (MAP1: f loc to fto1)
-    :
-      fto0 = fto1.
-  Proof.
-    hexploit deattached_memory_get_new; try apply MAP0; eauto. i. des.
-    hexploit deattached_memory_get_new; try apply MAP1; eauto. i. des. clarify.
-    exploit Memory.get_disjoint.
-    { eapply GETDNEW. }
-    { eapply GETDNEW0. } i. des; subst; auto.
-    exfalso. eapply x0.
-    { instantiate (1:=Time.meet fto0 fto1). unfold Time.meet. des_ifs.
-      - econs; ss. refl.
-      - econs; ss. left. auto. }
-    { unfold Time.meet. des_ifs. econs; ss. refl. }
-  Qed.
-
-  Lemma deattached_memory_map_inj
-        f mem mem_d
-        (DEATTACH: deattached_memory f mem mem_d)
-        loc to0 to1 fto
-        (MAP0: f loc to0 fto)
-        (MAP1: f loc to1 fto)
-    :
-      to0 = to1.
-  Proof.
-    hexploit deattached_memory_get_new; try apply MAP0; eauto. i. des.
-    hexploit deattached_memory_get_new; try apply MAP1; eauto. i. des. clarify.
-    exploit Memory.get_disjoint.
-    { eapply GETORIG. }
-    { eapply GETORIG0. } i. des; subst; auto.
-    exfalso. eapply x0.
-    { instantiate (1:=fto). econs; ss. left. auto. }
-    { econs; ss. left. auto. }
-  Qed.
-
-  Lemma deattached_memory_get_orig_unmap
-        f mem mem_d
-        (DEATTACH: deattached_memory f mem mem_d)
-        loc to fto
-        (MAP: f loc to fto)
-    :
-      Memory.get loc fto mem = None.
-  Proof.
-    hexploit deattached_memory_get_new; eauto. i. des.
-    destruct (Memory.get loc fto mem) as [[from' msg]|] eqn:GET; auto. exfalso.
-    exploit Memory.get_disjoint.
-    { eapply GETORIG. }
-    { eapply GET. } i. des; subst.
-    - eapply Time.lt_strorder; eauto.
-    - eapply x0.
-      + instantiate (1:=fto). econs; ss. left. auto.
-      + econs; ss.
-        * eapply memory_get_ts_strong in GET. des; subst; auto.
-          exfalso. eapply Time.lt_strorder. eapply TimeFacts.lt_le_lt.
-          { eapply TS0. }
-          { eapply Time.bot_spec. }
-        * refl.
-  Qed.
-
-  Lemma deattaching_promises
-        (self: Loc.t -> Time.t -> Prop) mem prom
-        (SELF: forall loc to (SELF: self loc to),
-            exists from,
-              (<<GET: Memory.get loc to prom = Some (from, Message.reserve)>>))
-        (MLE: Memory.le prom mem)
-        (FIN: Memory.finite prom)
-        (CLOSED: Memory.closed mem)
-    :
-      exists f mem' prom',
-        (<<FUTURE: reserve_future_memory prom mem prom' mem'>>) /\
-        (<<DEATTACHMEM: deattached_memory f mem mem'>>) /\
-        (<<DEATTACHPROM: deattached_memory f prom prom'>>) /\
-        (<<COMPLETE: forall loc to (SELF: self loc to),
-            exists fto, (<<MAP: f loc to fto>>)>>) /\
-        (<<SOUND: forall loc to fto (MAP: f loc to fto), self loc to>>).
-  Proof.
-    assert (exists (l: list (Loc.t * Time.t)),
-               (<<COMPLETE: forall loc to,
-                   self loc to <-> List.In (loc, to) l>>)).
-    { unfold Memory.finite in *. des.
-      hexploit list_filter_exists.
-      instantiate (2:=fun locto => self (fst locto) (snd locto)).
-      instantiate (1:=dom). i. des. exists l'.
-      i. split.
-      - i. eapply COMPLETE. splits; auto.
-        exploit SELF; eauto. i. des. eapply FIN; eauto.
-      - i. eapply COMPLETE in H. des. auto.
-    }
-    des. ginduction l.
-    { i. exists (fun _ _ _ => False), mem, prom. splits.
-      - econs 1.
-      - econs; i; ss.
-      - econs; i; ss.
-      - i. eapply COMPLETE in SELF0. ss.
-      - i. ss. }
-    { i. destruct a as [loc to].
-      destruct (classic (List.In (loc, to) l)) as [IN|NIN].
-      { eapply IHl; eauto. i. rewrite COMPLETE. ss.
-        split; i; auto. des; auto. clarify. }
-      hexploit (IHl L (fun loc' to' => (<<SELF: self loc' to'>>)
-                                       /\ (<<REMOVE: (loc, to) <> (loc', to')>>))); eauto.
-      { i. des. eauto. }
-      { i. split; i.
-        - des. eapply COMPLETE in SELF0. ss. des; auto. clarify.
-        - split.
-          + eapply COMPLETE. ss. auto.
-          + ii. clarify. }
-      i. des.
-
-      assert (SELFTS: self loc to).
-      { eapply COMPLETE. ss. auto. }
-      assert (NMAP0: forall fto, ~ f loc to fto).
-      { ii. eapply SOUND in H. des. clarify. }
-      assert (NMAP1: forall f_1to, ~ f loc f_1to to).
-      { ii. dup H. eapply SOUND in H. des.
-        hexploit (DEATTACHPROM.(deattached_memory_get_new)); eauto. i. des.
-        exploit SELF; try apply SELFTS. i. des.
-        exploit Memory.get_disjoint.
-        { eapply GET. }
-        { eapply GETORIG. }
-        i. des; subst; clarify. eapply x0.
-        { instantiate (1:=to). econs; ss.
-          - apply memory_get_ts_strong in GET. des; subst; auto.
-            exfalso. eapply Time.lt_strorder. eapply TimeFacts.lt_le_lt.
-            { eapply TS0. }
-            { eapply Time.bot_spec. }
-          - refl. }
-        { econs; ss. left. auto. }
-      }
-
-      hexploit SELF.
-      { eauto. } i. des.
-      rewrite DEATTACHPROM.(deattached_memory_get_normal) in GET; eauto.
-      assert (GETMEM: Memory.get loc to mem' = Some (from, Message.reserve)).
-      { eapply reserve_future_memory_le; eauto. }
-
-      assert (FROMTO: Time.lt from to).
-      { apply memory_get_ts_strong in GET. des; auto. subst.
-        exploit Memory.future_closed.
-        { eapply reserve_future_future; eauto. }
-        { eauto. }
-        intros []. erewrite INHABITED in GETMEM. clarify. }
-      set (fto := Time.middle from to).
-
-      hexploit (@Memory.remove_exists prom' loc from to Message.reserve); eauto.
-      intros [prom0 REMOVEPROM].
-      hexploit (@Memory.remove_exists_le prom' mem' loc from to Message.reserve); eauto.
-      { eapply reserve_future_memory_le; eauto. }
-      intros [mem0 REMOVEMEM].
-
-      assert (PROMISE0: Memory.promise prom' mem' loc from to Message.reserve prom0 mem0 Memory.op_kind_cancel).
-      { econs; eauto. }
-
-      hexploit (@Memory.add_exists mem0 loc from fto Message.reserve).
-      { ii. exploit Memory.get_disjoint.
-        { instantiate (4:=to2).
-          erewrite Memory.remove_o in GET2; eauto. des_ifs. eauto. }
-        { eapply GETMEM. }
-        i. des; subst.
-        { eapply Memory.remove_get0 in REMOVEMEM. des. clarify. }
-        { eapply x1; eauto. inv LHS. econs; ss.
-          transitivity fto; auto. left. eapply Time.middle_spec; auto. }
-      }
-      { eapply Time.middle_spec; eauto. }
-      { econs. }
-      intros [mem1 ADDMEM].
-      hexploit (@Memory.add_exists_le prom0 mem0 loc from fto Message.reserve); eauto.
-      { eapply promise_memory_le; cycle 1; eauto.
-        eapply reserve_future_memory_le; eauto. }
-      intros [prom1 ADDPROM].
-      assert (PROMISE1: Memory.promise prom0 mem0 loc from fto Message.reserve prom1 mem1 Memory.op_kind_add).
-      { econs; eauto. i. clarify. }
-
-      assert (NMAP2: forall fto', ~ f loc fto fto').
-      { i. intros MAP.
-        exploit deattached_memory_get_new; try apply DEATTACHPROM; eauto. i. des.
-        exploit Memory.get_disjoint.
-        { eapply GETORIG. }
-        { instantiate (3:=to).
-          erewrite deattached_memory_get_normal; try apply DEATTACHPROM; eauto. }
-        i. des.
-        { exfalso. eapply Time.lt_strorder.
-          instantiate (1:=to). rewrite <- x0 at 1.
-          eapply Time.middle_spec; auto. }
-        { eapply x0.
-          { instantiate (1:=fto). econs; ss.
-            - etrans; eauto.
-            - refl. }
-          { econs; ss.
-            - eapply Time.middle_spec; auto.
-            - left. eapply Time.middle_spec; auto. }
-        }
-      }
-
-      assert (NMAP3: forall to', ~ f loc to' fto).
-      { i. intros MAP.
-        exploit deattached_memory_get_new; try apply DEATTACHPROM; eauto. i. des.
-        exploit Memory.get_disjoint.
-        { eapply GETORIG. }
-        { instantiate (3:=to).
-          erewrite deattached_memory_get_normal; try apply DEATTACHPROM; eauto. }
-        i. des; subst.
-        { eapply NMAP0; eauto. }
-        { eapply x0.
-          { instantiate (1:=fto). econs; ss. left. auto. }
-          { econs; ss.
-            - eapply Time.middle_spec; auto.
-            - left. eapply Time.middle_spec; auto. }
-        }
-      }
-
-      exists (fun l t ft => (<<ORIG: f l t ft>>) \/ (<<NEW: l = loc /\ t = to /\ ft = fto>>)),
-      mem1, prom1. splits.
-      { eapply reserve_future_memory_trans; eauto. }
-      { econs.
-        { i. erewrite (@Memory.add_o mem1); eauto.
-          erewrite (@Memory.remove_o mem0); eauto. des_ifs.
-          - ss. des; clarify. exfalso.
-            eapply NMAP5; eauto.
-          - ss. des; clarify. exfalso.
-            eapply NMAP4; eauto.
-          - eapply deattached_memory_get_normal; eauto.
-            { ii. eapply NMAP4; eauto. }
-            { ii. eapply NMAP5; eauto. }
-        }
-        { i. des.
-          { exploit deattached_memory_get_new; try apply DEATTACHMEM; eauto. i. des. esplits; eauto.
-            - erewrite (@Memory.add_o mem1); eauto.
-              erewrite (@Memory.remove_o mem0); eauto. des_ifs.
-              + ss. des; clarify. exfalso. eapply NMAP3; eauto.
-              + ss. des; clarify. exfalso. eapply NMAP1; eauto.
-            - erewrite (@Memory.add_o mem1); eauto.
-              erewrite (@Memory.remove_o mem0); eauto. des_ifs.
-              ss. des; clarify. exfalso. eapply NMAP2; eauto.
-          }
-          { subst. exists from. splits; auto.
-            { erewrite deattached_memory_get_normal; try apply DEATTACHMEM; eauto. }
-            { eapply Memory.add_get0; eauto. }
-            { erewrite (@Memory.add_o mem1); eauto.
-              erewrite (@Memory.remove_o mem0); eauto. des_ifs.
-              - ss. des; clarify.
-                exfalso. eapply Time.lt_strorder.
-                instantiate (1:=to). rewrite a0 at 1. eapply Time.middle_spec; auto.
-              - ss. des; clarify. }
-            { eapply Time.middle_spec; eauto. }
-            { eapply Time.middle_spec; eauto. }
-          }
-        }
-      }
-      { econs.
-        { i. erewrite (@Memory.add_o prom1); eauto.
-          erewrite (@Memory.remove_o prom0); eauto. des_ifs.
-          - ss. des; clarify. exfalso.
-            eapply NMAP5; eauto.
-          - ss. des; clarify. exfalso.
-            eapply NMAP4; eauto.
-          - eapply deattached_memory_get_normal; eauto.
-            { ii. eapply NMAP4; eauto. }
-            { ii. eapply NMAP5; eauto. }
-        }
-        { i. des.
-          { exploit deattached_memory_get_new; try apply DEATTACHPROM; eauto. i. des. esplits; eauto.
-            - erewrite (@Memory.add_o prom1); eauto.
-              erewrite (@Memory.remove_o prom0); eauto. des_ifs.
-              + ss. des; clarify. exfalso. eapply NMAP3; eauto.
-              + ss. des; clarify. exfalso. eapply NMAP1; eauto.
-            - erewrite (@Memory.add_o prom1); eauto.
-              erewrite (@Memory.remove_o prom0); eauto. des_ifs.
-              ss. des; clarify. exfalso. eapply NMAP2; eauto.
-          }
-          { subst. exists from. splits; auto.
-            { erewrite deattached_memory_get_normal; try apply DEATTACHPROM; eauto. }
-            { eapply Memory.add_get0; eauto. }
-            { erewrite (@Memory.add_o prom1); eauto.
-              erewrite (@Memory.remove_o prom0); eauto. des_ifs.
-              - ss. des; clarify.
-                exfalso. eapply Time.lt_strorder.
-                instantiate (1:=to). rewrite a0 at 1. eapply Time.middle_spec; auto.
-              - ss. des; clarify. }
-            { eapply Time.middle_spec; eauto. }
-            { eapply Time.middle_spec; eauto. }
-          }
-        }
-      }
-      { i. destruct (classic ((loc0, to0) = (loc, to))).
-        - clarify. eauto.
-        - exploit COMPLETE0; eauto. i. des. eauto. }
-      { i. des.
-        - eapply SOUND in MAP. des. auto.
-        - subst. auto. }
-    }
-  Qed.
-
-  Definition attached_promises (self prom: Loc.t -> Time.t -> Prop) (mem: Memory.t)
-             (loc: Loc.t) (ts0: Time.t): Prop :=
-    (<<SELF: self loc ts0>>) /\
-    (<<ATTACH: exists ts1 msg,
-        (<<GET: Memory.get loc ts1 mem = Some (ts0, msg)>>) /\
-        (<<OTHERS: ~ prom loc ts1>>)>>).
-
-  Inductive mapped_self_promises (self: Loc.t -> Time.t -> Prop)
-            (f: Loc.t -> Time.t -> Time.t -> Prop)
-    :
-      forall (loc: Loc.t) (ts: Time.t), Prop:=
-  | mapped_self_promises_unmap
-      loc ts
-      (SELF: self loc ts)
-      (UNMAP: forall fts, ~ f loc ts fts)
-    :
-      mapped_self_promises self f loc ts
-  | mapped_self_promises_map
-      loc ts fts
-      (MAP: f loc ts fts)
-      (SELF: self loc ts)
-    :
-      mapped_self_promises self f loc fts
-  .
-
-  Inductive mid_map (mem: Memory.t) (prom: Memory.t)
-            (f: Loc.t -> Time.t -> Time.t -> Prop)
-    :
-      Loc.t -> Time.t -> Time.t -> Prop :=
-  | mid_map_normal
-      loc ts
-      (NMAP: forall fts, ~ f loc ts fts)
-      (PROMISED: promised mem loc ts)
-    :
-      mid_map mem prom f loc ts ts
-  | mid_map_promise
-      loc from to msg
-      (NMAP: forall fts, ~ f loc to fts)
-      (PROMISED: Memory.get loc to prom = Some (from, msg))
-    :
-      mid_map mem prom f loc from from
-  | mid_map_map
-      loc ts fts
-      (MAP: f loc ts fts)
-    :
-      mid_map mem prom f loc ts fts
-  .
-  Hint Constructors mid_map.
-
-  Lemma mid_map_map_bot f mem mem' prom
-        (DEATTACHMEM: deattached_memory f mem mem')
-        (CLOSED: Memory.closed mem)
-    :
-      mapping_map_bot (mid_map mem prom f).
-  Proof.
-    ii. econs 1.
-    - ii. exploit deattached_memory_get_new; eauto. i. des.
-      exfalso. eapply Time.lt_strorder. eapply TimeFacts.lt_le_lt.
-      { eapply TS1. }
-      { eapply Time.bot_spec. }
-    - inv CLOSED. econs; eauto.
-  Qed.
-
-  Lemma mid_map_map_lt f mem mem' prom
-        (DEATTACHMEM: deattached_memory f mem mem')
-    :
-      mapping_map_lt (mid_map mem prom f).
-  Proof.
-    ii. inv MAP0; inv MAP1.
-    - auto.
-    - auto.
-    - exploit deattached_memory_get_new; eauto. i. des. split.
-      + i. inv PROMISED. destruct msg.
-        exploit memory_get_from_mon.
-        { eapply GET. }
-        { eapply GETORIG. }
-        { eauto. }
-        i. eapply TimeFacts.le_lt_lt; eauto.
-      + i. etrans; eauto.
-    - auto.
-    - auto.
-    -
-
-      admit.
-    - exploit deattached_memory_get_new; eauto. i. des. split.
-      + i. etrans; eauto.
-      + i. inv PROMISED. destruct msg.
-        destruct (Time.le_lt_dec ft1 t0); auto. destruct l.
-        { exfalso. exploit memory_get_from_mon.
-          { eapply GET. }
-          { eapply GETORIG. }
-          { eauto. }
-          i. eapply Time.lt_strorder. eapply TimeFacts.le_lt_lt.
-          { eapply x0. }
-          { transitivity ft0; auto. }
-        }
-        { inv H0. exfalso. eapply NMAP; eauto. }
-    - admit.
-    - exploit deattached_memory_get_new; try apply MAP; eauto.
-      exploit deattached_memory_get_new; try apply MAP0; eauto. i. des.
-      destruct (Time.le_lt_dec t0 t1); cycle 1.
-      { split; i.
-        - exfalso. eapply Time.lt_strorder. transitivity t0; eauto.
-        - exploit memory_get_from_mon.
-          { eapply GETORIG0. }
-          { eapply GETORIG. }
-          { eauto. }
-          i. exfalso. eapply Time.lt_strorder. eapply TimeFacts.lt_le_lt.
-          { eapply TS3. } etrans.
-          { eapply x0. } etrans.
-          { left. eapply TS0. }
-          { left. auto. }
-      }
-      destruct l.
-      { split; i; auto.
-        exploit memory_get_from_mon.
-        { eapply GETORIG. }
-        { eapply GETORIG0. }
-        { eauto. }
-        i. etrans.
-        { eapply TS1. } eapply TimeFacts.le_lt_lt.
-        { eapply x0. }
-        { eauto. }
-      }
-      { inv H. clarify. hexploit deattached_memory_map_eq.
-        { eauto. }
-        { eapply MAP. }
-        { eapply MAP0. }
-        i. subst. split; i; exfalso; eapply Time.lt_strorder; eauto.
-      }
-  Admitted.
-
-  Lemma deattached_promises_not_attached (self: Loc.t -> Time.t -> Prop)
-        f prom mem prom' mem'
-        (MLE: Memory.le prom' mem')
-        (DEATTACHMEM: deattached_memory f mem mem')
-        (DEATTACHPROM: deattached_memory f prom prom')
-        (COMPLETE: forall loc to (SELF: attached_promises self (promised prom) mem loc to),
-            exists fto, (<<MAP: f loc to fto>>))
-    :
-      promises_not_attached (mapped_self_promises self f) (promised prom') mem'.
-  Proof.
-    ii. inv PROMISED.
-    - admit.
-    - hexploit deattached_memory_get_new; try apply DEATTACHMEM; eauto. i. des.
-  Admitted.
 
 End MIDDLE.
